coding

300 ANU Computing/Theoretical Computer Science/dafny/week7_tutorial.dfy
@@ -1,11 +1,12 @@
 datatype Tree = Emp | Node (left_node: Tree, i_main_node: int, right_node: Tree)
 
-function is_in (i: int, t: Tree): bool {
-match t {
-    case Emp => false
-    case Node (left_node, j, right_node) => i == j ||
-        is_in(i, left_node) || is_in (i, right_node)
-} }
+function is_in (i_main_node: int, tree: Tree): bool {
+    match tree {
+        case Emp => false
+        case Node (left_node, j, right_node) => i_main_node == j ||
+            is_in(i_main_node, left_node) || is_in (i_main_node, right_node)
+    }
+}
 
 // passing in some integer 'i' and we want to see if it's in the Tree passed in.
 // if the list is empty, then it's not going to be in the list, so we return false
@@ -16,3 +17,112 @@ match t {
 // if the current node is null, then that ends.
 // we do the same on the right side, and we can find if something is
 // in the tree.
+
+
+
+function lookup (target: int, tree: Tree) : bool {
+    match tree {
+        case Emp => false
+        case Node (left_node, i_main_node, right_node) => 
+        (i_main_node == target) ||
+        (target < i_main_node && lookup(target,left_node)) || 
+        (target > i_main_node && lookup(target,right_node))
+    }
+}
+
+// Same as the above function, just doing it a different way.
+// function takes in an int 'j' and a tree 't'
+// the difference is how we go down the lists.
+// it's very similar, this is just more efficient,
+// as it only goes down the paths that is has to.
+
+// I.E., if the target is 17, instead of going through all of the
+// of the rows, it will just go through the right side,
+// and it will find it in like 3 iterators, as opposed to 10.
+//               14
+//          /          \
+//        6            18
+//      /   \        /     \
+//   3       nil   17       22
+// 
+
+
+// Binary Search Tree
+ghost predicate is_bst (tree: Tree) {
+    match tree {
+        case Emp => true
+        case Node (left_node, i_main_node, right_node) => 
+        // we are checking if the values are less than the 
+        // main node as this is a quality of 
+        (forall target: int :: is_in (target, left_node) ==> 
+            target < i_main_node) &&
+        (forall target: int :: is_in (target, right_node) ==> 
+            target > i_main_node) && 
+        is_bst(left_node) && is_bst(right_node)
+    }
+}
+// Returns either true or false.
+// A binary search tree is simply a data structure that follows these rules:
+// The left and side and the right hand side are balanced (+ - 1)
+// otherwise, you should reshape
+//                      07                     
+//                      /\                      this is an example of a binary search tree.
+//                     /  \                     it's used for optimising lookup times.
+//                    /    \                    there are a couple of things we have to check.
+//                   /      \                  1. if the nodes L and R are greater than the
+//                  /        \                  child nodes. This should not be the case.
+//                 /          \                2. If the parents node is longer than the
+//                /            \                r or l subtree
+//               /              \              3. If there are any duplicate values.
+//              /                \             
+//             /                  \            
+//            /                    \           
+//          03                      11         
+//          /\                      /\         
+//         /  \                    /  \        
+//        /    \                  /    \       
+//       /      \                /      \      
+//      /        \              /        \     
+//    01          05          09          13   
+//    /\          /\          /\          /\   
+//   /  \        /  \        /  \        /  \  
+// 00    02    04    06    08    10    12    14
+
+
+// Exercise 1
+// Formulate a lemma is in lookup that states that – for a binary search tree – the lookup function 
+// delivers the same result as is in (Dafny proves this automatically.) Give a proof of the statement 
+// by hand, stating clearly what you proved, the inductive hypothesis, the base case and the step case.
+// Now consider the function insert and the lemma insert bst.
+
+
+lemma {:induction false} is_in_lookup(tree: Tree, target: int)
+    requires is_bst(tree)
+    ensures (is_in(target, tree)) == (is_in(target, tree)){
+        // match tree{
+        //     case Emp => 
+        //     case Node (left_node, i_main_node, right_node) =>  
+        // }
+    }
+
+
+
+// Given functions
+function insert (j: int, t: Tree): Tree {
+    match t { case Emp => Node (Emp, j, Emp)
+        case Node (l, i, r) =>
+        if (j < i) then Node (insert (j, l), i, r)
+        else if (j > i) then Node (l, i, insert (j, r)) else t
+    }
+}
+
+lemma insert_bst (j: int, t: Tree)
+requires is_bst (t)
+ensures is_bst (insert (j, t))
+
+
+// Exercise 2 Insertion – Elements
+// Formulate two lemmas, insert is in and insert only in that assert that both j and 
+// every element i of a tree t are elements of insert(j, t), and that every element of 
+// insert (j, t) is of this form. Dafny should prove these lemmas automatically. As in 
+// the previous Exercise, also give the proof of insert is in by hand in a comment.
